msl_application/GList.v
@@ -108,4 +108,77 @@ Section GRAPH_GList.
     - apply (FiniteGraph_EnumCovered G), finGraph.
   Defined.
 
+  Definition single_uf_pregraph (v: addr) : PreGraph addr (addr * unit) :=
+    pregraph_add_edge (single_vertex_pregraph v) (v, tt) v v.
+
+  Lemma single_uf_is_uf: forall v, uf_graph (single_uf_pregraph v).
+  Proof.
+    intros. hnf. intros. hnf. exists (v, nil). split.
+    - hnf. auto.
+    - intros. hnf in H1. hnf in H. subst v. destruct H1 as [[v p] [[? ?] [? ?]]]. simpl in H. subst v. destruct p.
+      + simpl in *. subst y. exists (x, nil). split.
+        * hnf. split; [split; split|]; simpl; auto.
+          intros. destruct H as [[? ?] [? ?]]. clear H5. destruct x'. simpl in H. subst a. destruct l. auto.
+          destruct H4 as [_ ?]. destruct p. simpl in H. destruct l.
+          -- hnf in H. simpl in H. unfold updateEdgeFunc in H. destruct H as [_ [_ ?]].
+             destruct (equiv_dec (x, tt) (a, u)); destruct (equiv_dec x x); [|hnf in c | |hnf in c]; exfalso; auto.
+          -- unfold updateEdgeFunc in H. destruct H as [_ [? _]].
+             assert ((if equiv_dec (x, tt) p then x else x) = x) by (destruct (equiv_dec (x, tt) p); auto). rewrite H4 in H. clear H4.
+             destruct (equiv_dec (x, tt) (a, u)); destruct (equiv_dec x x); [|hnf in c| | hnf in c]; exfalso; auto.
+        * apply Subpath_refl.
+      + exfalso. clear H3. simpl in H0. simpl in H2. destruct H2 as [_ ?]. destruct p0.
+        * hnf in H. simpl in H. unfold updateEdgeFunc in H. destruct H as [_ [_ ?]].
+          destruct (equiv_dec (x, tt) p); destruct (equiv_dec x x); [|hnf in c| | hnf in c]; exfalso; auto.
+        * unfold updateEdgeFunc in H. destruct H as [_ [? _]].
+          assert ((if equiv_dec (x, tt) p0 then x else x) = x) by (destruct (equiv_dec (x, tt) p0); auto). rewrite H2 in H. clear H2.
+          destruct (equiv_dec (x, tt) p); destruct (equiv_dec x x); [|hnf in c| | hnf in c]; exfalso; auto.
+  Qed.
+
+  Lemma reachabel_single_uf: forall x y, reachable (single_uf_pregraph x) x y <-> x = y.
+  Proof.
+    intros. split; intros.
+    - destruct H as [[? ?] [[? ?] [? _]]]. simpl in H. subst a. induction l.
+      + simpl in H0. auto.
+      + destruct a as [? ?].
+        assert (a = x). {
+          clear H0 IHl. simpl in H1. destruct l.
+          - destruct H1 as [_ ?]. hnf in H. simpl in H. unfold addValidFunc in H. destruct H as [[? | ?] _]; [exfalso | inversion H]; auto.
+          - destruct H1 as [_ [? _]]. hnf in H. simpl in H. unfold addValidFunc in H. destruct H as [[? | ?] _]; [exfalso | inversion H]; auto.
+        } subst a. rewrite pfoot_cons in H0. apply valid_path_cons in H1.
+        assert (dst (single_uf_pregraph x) (x, u) = x) by (simpl; unfold updateEdgeFunc; destruct (equiv_dec (x, tt) (x, u)); auto). rewrite H in *.
+        apply IHl; auto.
+    - subst y. apply reachable_refl. simpl. auto.        
+  Qed.
+
+  Definition single_uf_LabeledGraph (v: addr) (default_dv: DV) (default_de: DE) (default_dg: DG) : LGraph :=
+    Build_LabeledGraph _ _ _ (single_uf_pregraph v) (fun v => default_dv) (fun e => default_de) default_dg.
+
+  Definition single_uf_MathGraph (v: addr) (H: v <> null): MathGraph (single_uf_pregraph v) is_null_SGBA.
+  Proof.
+    apply (Build_MathGraph _ is_null_SGBA).
+    - intros. simpl. unfold updateEdgeFunc.
+      destruct (equiv_dec (v, tt) e); intuition.
+    - intros. hnf in *. subst v. intuition.
+  Defined.
+
+  Definition single_uf_FiniteGraph (v: addr): FiniteGraph (single_uf_pregraph v).
+  Proof.
+    constructor; hnf.
+    - exists (v :: nil). split.
+      + constructor. intro. inversion H. constructor.
+      + intros. simpl. unfold In. intuition.
+    - exists ((v, tt) :: nil). split.
+      + constructor. intro. inversion H. constructor.
+      + intros. simpl. unfold In, addValidFunc. intuition.
+  Defined.
+
+  Definition single_uf_LstGraph (v: addr): LstGraph (single_uf_pregraph v) (fun x => (x, tt)).
+  Proof. constructor; simpl; intros. unfold updateEdgeFunc, addValidFunc. subst. destruct (equiv_dec (x, tt) e); intuition. Defined.
+
+  Definition single_sound (v: addr) (H: v <> null) : LiMaFin (single_uf_pregraph v) :=
+    Build_LiMaFin _ (single_uf_LstGraph v) (single_uf_MathGraph v H) (single_uf_FiniteGraph v).
+    
+  Definition single_Graph (v: addr) (H: v <> null) (default_dv: DV) (default_de: DE) (default_dg: DG): Graph :=
+    Build_GeneralGraph _ _ _ _ (single_uf_LabeledGraph v default_dv default_de default_dg) (single_sound v H).
+
 End GRAPH_GList.
